Get typed_fs infrastructure working

src/Dafny/examples/fs/typed_fs.dfy
@@ -1,6 +1,8 @@
 include "byte_fs.dfy"
 
 module TypedFs {
+  import opened Std
+
   import opened ByteFs
   import opened FsKinds
   import opened JrnlTypes
@@ -34,8 +36,16 @@ module TypedFs {
       && fs.fs.ValidIno(ino, i)
     }
 
+    lemma reveal_valids()
+      ensures bytefsValid() == fs.fs.Valid()
+      ensures forall ino:Ino, i :: fsValidIno(ino, i) == fs.fs.ValidIno(ino, i)
+    {
+      reveal bytefsValid();
+      reveal fsValidIno();
+    }
+
     predicate {:opaque} ValidFields()
-      reads Repr
+      reads this, fs.Repr
       requires bytefsValid()
     {
       reveal bytefsValid();
@@ -120,5 +130,85 @@ module TypedFs {
     {
       fs.fs.has_jrnl(txn)
     }
+
+    predicate inode_unmodified(ino: Ino, i: Inode.Inode)
+      reads fs.fs.fs
+    {
+      fs.fs.fs.cur_inode == Some((ino, i))
+    }
+
+    method startInode(txn: Txn, ino: Ino) returns (i': Inode.Inode)
+      modifies fs.fs.fs
+      requires has_jrnl(txn)
+      requires Valid() ensures ValidIno(ino, i')
+      ensures inode_unmodified(ino, i')
+    {
+      reveal_valids();
+      i' := fs.startInode(txn, ino);
+      reveal ValidFields();
+    }
+
+    ghost method finishInodeReadonly(ino: Ino, i: Inode.Inode)
+      modifies fs.fs.fs
+      requires ValidIno(ino, i)
+      requires inode_unmodified(ino, i)
+      ensures Valid()
+    {
+      reveal_valids();
+      fs.finishInodeReadonly(ino, i);
+      reveal ValidFields();
+    }
+
+    method finishInode(txn: Txn, ino: Ino, i: Inode.Inode)
+      modifies fs.Repr
+      requires has_jrnl(txn)
+      requires ValidIno(ino, i)
+      ensures Valid()
+    {
+      reveal_valids();
+      fs.finishInode(txn, ino, i);
+      reveal ValidFields();
+    }
+
+    lemma inode_metadata(ino: Ino, i: Inode.Inode)
+      requires ValidIno(ino, i)
+      ensures i.meta.ty == types[ino]
+      ensures i.meta.sz as nat == |data[ino]|
+    {
+      fs.inode_metadata(ino, i);
+      reveal ValidFields();
+    }
+
+    method allocInode(txn: Txn, ty: Inode.InodeType) returns (ok: bool, ino: Ino, i: Inode.Inode)
+      modifies Repr
+      requires Valid()
+      requires has_jrnl(txn)
+      ensures ok ==>
+      && old(types[ino].InvalidType?) && types == old(types[ino := ty])
+      && data == old(data)
+      && data[ino] == []
+      && ValidIno(ino, i)
+    {
+      ino := ialloc.Alloc();
+      i := startInode(txn, ino);
+      inode_metadata(ino, i);
+      if !i.meta.ty.InvalidType? {
+        ok := false;
+        return;
+      }
+      i := fs.setType(ino, i, ty);
+      types := fs.inode_types();
+      reveal ValidInvalid();
+      reveal ValidFields();
+    }
+
+    // todo
+      // fs.alignedWrite
+      // fs.appendIno
+      // fs.readInternal
+      // fs.readWithInode
+      // fs.setSize
+      // fs.shrinkToEmpty
+
   }
 }
